src/program_proof/lockservice/lockservice_proof.v
@@ -7,7 +7,7 @@ From Perennial.algebra Require Import auth_map.
 From Perennial.goose_lang Require Import notation.
 From Perennial.goose_lang.lib Require Import lock.
 From Perennial.program_proof Require Import proof_prelude.
-From Perennial.program_proof.lockservice Require Import lockservice rpc common_proof nondet.
+From Perennial.program_proof.lockservice Require Import lockservice rpc_proof nondet.
 
 Record lockservice_names := LockserviceNames {
   ls_rpcGN : rpc_names;
